simplify
git-svn-id: https://projects.brucker.ch/hol-testgen/svn/HOL-TestGen/trunk/hol-testgen@13500 3260e6d1-4efc-4170-b0a7-36055960796d

src/compiler/meta/Meta_HKB.thy
@@ -41,7 +41,13 @@ section\<open>Isabelle Meta-Model aka. AST definition of Isabelle\<close>
 theory Meta_HKB
 imports "../../compiler_generic/Init"
 begin
- 
+
+section \<open>Miscellaneous\<close>
+
+datatype gen_meta = Gen_apply_hol string (* HOL term to apply *)
+                  | Gen_apply_sml string (* SML term to apply *)
+                  | Gen_no_apply
+
 section \<open>Isa.hs\<close>
 
 (* Author: Tobias C. Rittweiler, TU Muenchen
@@ -116,7 +122,7 @@ Conversion from abstract Haskell code to abstract Isar/HOL theory.
 
 datatype IsaUnit = IsaUnit "bool (* true: generate with 'old_datatype' instead of 'datatype' *) \<times> nat (* 0: full datatype, \<ge> 1: more atomic *)" (* FIXME add a generic meta-command 'generation_syntax_params' to parameterize at any interleaving place the generating mode (i.e. datatype or old_datatype) *)
                            "(string (* old prefix name to replace *) \<times> string option (* new substitute (or none to remove the prefix) *)) list"
-                           "(bool (* true: meta *) \<times> string (* converting function to apply once the parsed value is created *)) option"
+                           gen_meta (* converting function to apply once the parsed value is created *)
                            string (* name of the current theory *) (* FIXME move that 'static value' to the global environment. In principle, each meta-command is evaluated within one "own" theory name, following the hierarchy of children theories... *)
                            "Module list \<times> bool (* true: treat as most the list as a single module *)"
 
